Finish proofs for mapping_db functions

AssocList.v
@@ -1,537 +1,846 @@
 Require Import NArith.
 Require Import List.
 
-Section AssocListDef.
-
-Variable T : Type.
-
 (** An association list is a mapping between keys, which are natural numbers, and
     values of an arbitrary type. There is at most one value per key. *)
-Definition assoc_list : Type := list (N * T).
+Definition assoc_list (T:Type) : Type := list (N * T).
 
-Set Contextual Implicit.
-Definition empty : assoc_list := nil.
-Global Arguments empty : default implicits.
+Section InDomain.
 
-Fixpoint remove (k:N) (l:assoc_list) : assoc_list :=
-  match l with
-    | nil    => nil
-    | h :: t => let (k',v) := h in if N.eq_dec k' k then t else h :: remove k t
-  end.
-Global Arguments remove : default implicits.
+  Variable T : Type.
 
-Definition insert (k:N) (v:T) (l:assoc_list) : assoc_list :=
-  (k,v) :: remove k l.
-Global Arguments insert : default implicits.
+  Definition in_domain (k:N) (l:assoc_list T) : Prop := exists v, In (k,v) l.
+  Global Arguments in_domain : default implicits.
 
-Fixpoint assoc (k:N) (l:assoc_list) : option T :=
-  match l with
-    | nil    => None
-    | h :: t => if N.eq_dec (fst h) k then Some (snd h) else assoc k t
-  end.
-Global Arguments assoc : default implicits.
+  Theorem In_in_domain :
+    forall (l:assoc_list T) (k:N) (v:T), In (k,v) l -> in_domain k l.
+  Proof. Hint Unfold in_domain. eauto. Qed.
 
-End AssocListDef.
+  Theorem not_in_domain_In :
+    forall (l:assoc_list T) (k:N) (v:T), ~in_domain k l -> ~In (k,v) l.
+  Proof. Hint Unfold in_domain not. eauto. Qed.
 
-Section InvariantDef.
+  Lemma in_domain_inv :
+    forall (k:N) (k':N) (v:T) (l:assoc_list T),
+      in_domain k ((k',v) :: l) <-> k' = k \/ in_domain k l.
+  Proof.
+    Hint Resolve in_cons in_eq.
+    unfold in_domain. intros. split.
+    - destruct 1 as [v' in_l]. apply in_inv in in_l. destruct in_l.
+      + inversion H. subst. tauto.
+      + eauto.
+    - destruct 1 as [ke | [v' in_l]]; subst; eauto.
+  Qed.
 
-Variable T : Type.
+  Lemma in_domain_inv_tail :
+    forall (k k':N) (v:T) (l:assoc_list T),
+      k' <> k -> (in_domain k ((k',v) :: l) <-> in_domain k l).
+  Proof.
+    intros k k' v l ineq. split.
+    - intros H. apply in_domain_inv in H. destruct H; [contradiction | assumption].
+    - intros. apply in_domain_inv. auto.
+  Qed.
 
-Definition contains (k:N) (P:T -> Prop) (l:assoc_list T) : Prop :=
-  exists v, In (k,v) l /\ P v.
+  Lemma not_in_domain_inv :
+    forall (k k':N) (v:T) (l:assoc_list T),
+      ~in_domain k ((k',v) :: l) -> k <> k' /\ ~in_domain k l.
+  Proof.
+    unfold not. unfold in_domain. split; destruct 1; eauto.
+  Qed.
 
-Lemma contains_inv :
-  forall (k:N) (P:T -> Prop) (k':N) (v:T) (l:assoc_list T),
-    contains k P ((k',v) :: l) <-> (k' = k /\ P v) \/ contains k P l.
-Proof.
-  Hint Resolve in_eq in_cons.
-  intros k P k' v l. unfold contains. split.
-  - destruct 1 as [v' [in_k HP]]. apply in_inv in in_k. destruct in_k.
-    + inversion H. subst. tauto.
-    + eauto.
-  - destruct 1 as [[ke HP]|[v' [v'_in HP]]]; subst; intuition eauto.
-Qed.
+  Theorem not_in_domain_cons :
+    forall (l:assoc_list T) (k k':N) (v:T),
+      k <> k' -> ~in_domain k l -> ~in_domain k ((k',v) :: l).
+  Proof.
+    unfold in_domain. intros l k k' v ineq not_in_l.
+    destruct 1 as [? [E|E]]; [inversion E|]; eauto.
+  Qed.
 
-Lemma contains_app_or :
-  forall (k:N) (P:T -> Prop) (l1 l2:assoc_list T),
-    contains k P (l1 ++ l2) <-> contains k P l1 \/ contains k P l2.
-Proof.
-  Hint Resolve in_or_app .
-  unfold contains.
-  intros k P l1 l2. split.
-  - destruct 1 as [v [in_l12 HP]]. apply in_app_or in in_l12. intuition eauto.
-  - destruct 1 as [in_l|in_l]; destruct in_l as [v [in_l HP]]; eauto.
-Qed.
+  Lemma in_domain_app_or :
+    forall (k:N) (l1 l2:assoc_list T),
+      in_domain k (l1 ++ l2) <-> in_domain k l1 \/ in_domain k l2.
+  Proof.
+    Hint Resolve in_or_app.
+    unfold in_domain.
+    intros k l1 l2. split.
+    - destruct 1 as [v in_l12]. apply in_app_or in in_l12. intuition eauto.
+    - destruct 1 as [in_l|in_l]; destruct in_l as [v in_l]; eauto.
+  Qed.
 
-Definition in_domain (k:N) : assoc_list T -> Prop := contains k (fun _ => True).
+  Lemma not_in_domain_nil :
+    forall (k:N), ~in_domain k nil.
+  Proof.
+    intros. unfold in_domain. destruct 1. auto.
+  Qed.
 
-Theorem contains_in_domain :
-  forall (l:assoc_list T) (k:N) (P:T -> Prop), contains k P l -> in_domain k l.
-Proof.
-  unfold in_domain. unfold contains. intros l k P. destruct 1. intuition eauto.
-Qed.
+  Theorem in_domain_dec : forall (l:assoc_list T) (k:N), in_domain k l + ~in_domain k l.
+  Proof.
+    Hint Resolve not_in_domain_nil not_in_domain_cons in_cons.
+    Hint Unfold in_domain.
+    intros l k. induction l as [|[k' v] t IH].
+    - eauto.
+    - destruct IH as [H | not_in_t].
+      + left. destruct H. eauto.
+      + destruct (N.eq_dec k' k); subst; eauto.
+  Qed.
 
-Lemma in_domain_inv :
-  forall (k:N) (k':N) (v:T) (l:assoc_list T),
-    in_domain k ((k',v) :: l) <-> k' = k \/ in_domain k l.
-Proof. unfold in_domain. intros. rewrite contains_inv. tauto. Qed.
+End InDomain.
 
-Theorem in_domain_contains_eq :
-  forall (l:assoc_list T) (k:N), in_domain k l -> exists v, contains k (eq v) l.
-Proof.
-  Hint Resolve in_domain_inv in_nil.
-  intros l k. induction l as [|[k' v] t IH].
-  - destruct 1. exfalso. intuition auto.
-  - unfold in_domain. unfold contains. destruct 1 as [v' [k_in _]].
-    apply in_inv in k_in. case k_in.
-    + inversion 1. subst. eauto.
-    + eauto.
-Qed.
+Section Disjoint.
 
-Lemma in_domain_app_or :
-  forall (k:N) (l1 l2:assoc_list T),
-    in_domain k (l1 ++ l2) <-> in_domain k l1 \/ in_domain k l2.
-Proof. unfold in_domain. intros. rewrite contains_app_or. tauto. Qed.
+  Variable T : Type.
 
-Definition al_disjoint (l1 l2:assoc_list T) : Prop :=
-  forall k, in_domain k l1 -> ~in_domain k l2.
+  Definition al_disjoint (l1 l2:assoc_list T) : Prop :=
+    forall k, in_domain k l1 -> ~in_domain k l2.
+  Global Arguments al_disjoint : default implicits.
 
-Lemma al_disjoint_nil_l :
-  forall (l1:assoc_list T), al_disjoint nil l1.
-Proof.
-  intros l1 k. unfold in_domain. unfold contains. destruct 1 as [v [in_nil HP]].
-  contradiction.
-Qed.
+  Lemma al_disjoint_nil_l :
+    forall (l1:assoc_list T), al_disjoint nil l1.
+  Proof.
+    intros l1 k. unfold in_domain. destruct 1 as [v in_nil]. contradiction.
+  Qed.
 
-Lemma al_disjoint_symmetry :
-  forall (l1 l2:assoc_list T), al_disjoint l1 l2 -> al_disjoint l2 l1.
-Proof. unfold al_disjoint. eauto. Qed.
+  Lemma al_disjoint_symmetry :
+    forall (l1 l2:assoc_list T), al_disjoint l1 l2 -> al_disjoint l2 l1.
+  Proof. unfold al_disjoint. eauto. Qed.
 
-Lemma al_disjoint_cons_not_elem :
-  forall (l1 l2:assoc_list T) (k:N) (v:T),
-    ~(in_domain k l2) /\ al_disjoint l1 l2 <-> al_disjoint ((k,v) :: l1) l2.
-Proof.
-  Hint Resolve in_eq.
-  Hint Resolve <- in_domain_inv.
-  intros l1 l2 k v. split.
-  - unfold al_disjoint. destruct 1. intro. rewrite in_domain_inv.
-    destruct 1; subst; eauto.
-  - unfold al_disjoint. intros H. split; intros; try (apply H); eauto.
-Qed.
+  Lemma al_disjoint_cons_not_elem :
+    forall (l1 l2:assoc_list T) (k:N) (v:T),
+      ~(in_domain k l2) /\ al_disjoint l1 l2 <-> al_disjoint ((k,v) :: l1) l2.
+  Proof.
+    Hint Resolve in_eq.
+    Hint Resolve <- in_domain_inv.
+    intros l1 l2 k v. split.
+    - unfold al_disjoint. destruct 1. intro. rewrite in_domain_inv.
+      destruct 1; subst; eauto.
+    - unfold al_disjoint. intros H. split; intros; try (apply H); eauto.
+  Qed.
 
-Inductive al_invariant : assoc_list T -> Prop :=
-  | al_invariant_nil  : al_invariant nil
-  | al_invariant_cons :
-      forall (k:N) (v:T) (t:assoc_list T),
-        ~in_domain k t -> al_invariant t -> al_invariant ((k,v) :: t).
+End Disjoint.
 
-Lemma al_invariant_disjoint :
-  forall (l1 l2:assoc_list T), al_invariant (l1 ++ l2) -> al_disjoint l1 l2.
-Proof.
-  intros l1 l2 H. induction l1 as [|h t IH].
-  - apply al_disjoint_nil_l.
-  - destruct h as [k v]. apply al_disjoint_cons_not_elem. split.
-    + inversion H as [|k' v' t' not_in_tl2 inv_tl2]. subst.
-      rewrite in_domain_app_or in not_in_tl2. auto.
-    + apply IH. inversion H. assumption.
-Qed.
+Section Invariant.
 
-Lemma al_invariant_app_split :
-  forall (l1 l2:assoc_list T),
-    al_invariant (l1 ++ l2) -> al_invariant l1 /\ al_invariant l2.
-Proof.
-  Hint Constructors al_invariant.
-  Hint Resolve <- in_domain_app_or.
-  intros l1 l2 H. induction l1 as [|h t IH].
-  - auto.
-  - destruct h as [k v]. inversion H as [|k' v' t' not_in_tl2 inv_tl2]; subst. split;
-      try (apply al_invariant_cons);
-      intuition eauto.
-Qed.
+  Variable T : Type.
 
-Lemma al_invariant_join_app :
-  forall (l1 l2:assoc_list T),
-    al_invariant l1 -> al_invariant l2 -> al_disjoint l1 l2 -> al_invariant (l1 ++ l2).
-Proof.
-  intros l1 l2 inv_l1 inv_l2 dis. induction l1 as [|h t IH].
-  - assumption.
-  - destruct h as [k v]. simpl.
-    inversion inv_l1. subst.
-    apply <- al_disjoint_cons_not_elem in dis.
-    apply al_invariant_cons.
-    + rewrite in_domain_app_or. intuition auto.
-    + apply IH; tauto.
-Qed.
+  Inductive al_invariant : assoc_list T -> Prop :=
+    | al_invariant_nil  : al_invariant nil
+    | al_invariant_cons :
+        forall (k:N) (v:T) (t:assoc_list T),
+          ~in_domain k t -> al_invariant t -> al_invariant ((k,v) :: t).
+  Global Arguments al_invariant : default implicits.
 
-Lemma al_invariant_app_comm :
-  forall (l1 l2:assoc_list T), al_invariant (l1 ++ l2) -> al_invariant (l2 ++ l1).
-Proof.
-  intros l1 l2 H. apply al_invariant_join_app.
-  - apply al_invariant_app_split in H. apply H.
-  - apply al_invariant_app_split in H. apply H.
-  - apply al_invariant_disjoint in H. apply al_disjoint_symmetry. apply H.
-Qed.
+  Lemma al_invariant_disjoint :
+    forall (l1 l2:assoc_list T), al_invariant (l1 ++ l2) -> al_disjoint l1 l2.
+  Proof.
+    intros l1 l2 H. induction l1 as [|h t IH].
+    - apply al_disjoint_nil_l.
+    - destruct h as [k v]. apply al_disjoint_cons_not_elem. split.
+      + inversion H as [|k' v' t' not_in_tl2 inv_tl2]. subst.
+        rewrite in_domain_app_or in not_in_tl2. auto.
+      + apply IH. inversion H. assumption.
+  Qed.
 
-Lemma al_invariant_in_eq :
-  forall (l:assoc_list T) (k:N) (v v':T),
-    al_invariant l -> In (k,v) l -> In (k,v') l -> v = v'.
-Proof.
-  Hint Resolve in_inv contains_in_domain.
-  Hint Unfold contains in_domain not.
-  intros l k v v' inv_l v_in v'_in. induction l as [|[k' v''] t IH].
-  - destruct v_in.
-  - inversion inv_l. subst. case v_in.
-    + inversion 1. subst. case v'_in.
-      * inversion 1. auto.
-      * intros. exfalso. eauto 6.
-    + intros. case v'_in.
-      * inversion 1. subst. exfalso. eauto 6.
-      * auto.
-Qed.
+  Lemma al_invariant_app_split :
+    forall (l1 l2:assoc_list T),
+      al_invariant (l1 ++ l2) -> al_invariant l1 /\ al_invariant l2.
+  Proof.
+    Hint Constructors al_invariant.
+    Hint Resolve <- in_domain_app_or.
+    intros l1 l2 H. induction l1 as [|h t IH].
+    - auto.
+    - destruct h as [k v]. inversion H as [|k' v' t' not_in_tl2 inv_tl2]; subst. split;
+        try (apply al_invariant_cons);
+        intuition eauto.
+  Qed.
 
-Lemma contains_combine :
-  forall (l:assoc_list T) (k:N) (P1 P2:T -> Prop),
-    al_invariant l -> contains k P1 l -> contains k P2 l ->
-    contains k (fun x => P1 x /\ P2 x) l.
-Proof.
-  Hint Resolve al_invariant_in_eq.
-  unfold contains.
-  intros l k P1 P2 inv_l c_P1 c_P2.
-  destruct c_P1 as [v [in1 HP1]].
-  destruct c_P2 as [v' [in2 HP2]].
-  assert (eq: v' = v); subst; eauto.
-Qed.
+  Lemma al_invariant_join_app :
+    forall (l1 l2:assoc_list T),
+      al_invariant l1 -> al_invariant l2 -> al_disjoint l1 l2 -> al_invariant (l1 ++ l2).
+  Proof.
+    intros l1 l2 inv_l1 inv_l2 dis. induction l1 as [|h t IH].
+    - assumption.
+    - destruct h as [k v]. simpl.
+      inversion inv_l1. subst.
+      apply <- al_disjoint_cons_not_elem in dis.
+      apply al_invariant_cons.
+      + rewrite in_domain_app_or. intuition auto.
+      + apply IH; tauto.
+  Qed.
 
-End InvariantDef.
+  Lemma al_invariant_app_comm :
+    forall (l1 l2:assoc_list T), al_invariant (l1 ++ l2) -> al_invariant (l2 ++ l1).
+  Proof.
+    intros l1 l2 H. apply al_invariant_join_app.
+    - apply al_invariant_app_split in H. apply H.
+    - apply al_invariant_app_split in H. apply H.
+    - apply al_invariant_disjoint in H. apply al_disjoint_symmetry. apply H.
+  Qed.
+
+  Lemma al_invariant_in_eq :
+    forall (l:assoc_list T) (k:N) (v v':T),
+      al_invariant l -> In (k,v) l -> In (k,v') l -> v = v'.
+  Proof.
+    Hint Resolve in_inv In_in_domain.
+    Hint Unfold in_domain not.
+    intros l k v v' inv_l v_in v'_in. induction l as [|[k' v''] t IH].
+    - destruct v_in.
+    - inversion inv_l. subst. case v_in.
+      + inversion 1. subst. case v'_in.
+        * inversion 1. auto.
+        * intros. exfalso. eauto.
+      + intros. case v'_in.
+        * inversion 1. subst. exfalso. eauto.
+        * auto.
+  Qed.
+
+  Lemma in_eq_inv :
+    forall (l:assoc_list T) (k:N) (v v':T),
+      ~in_domain k l -> In (k,v) ((k,v') :: l) -> v = v'.
+  Proof.
+    intros l k v v' H. destruct 1 as [E|E]; [inversion E|exfalso]; eauto.
+  Qed.
+
+  Lemma in_cons_inv :
+    forall (l:assoc_list T) (k k':N) (v v':T),
+      k <> k' -> In (k',v') ((k,v) :: l) -> In (k',v') l.
+  Proof.
+    intros l k k' v v' ineq. destruct 1 as [E|E]; [inversion E; exfalso|]; eauto.
+  Qed.
+
+End Invariant.
+
+Section Contains.
+
+  Variable T : Type.
+
+  Definition contains (k:N) (P:T -> Prop) (l:assoc_list T) : Prop :=
+    exists v, In (k,v) l /\ P v.
+  Global Arguments contains : default implicits.
+
+  Theorem In_contains :
+    forall (k:N) (P:T -> Prop) (v:T) (l:assoc_list T),
+      In (k,v) l -> P v -> contains k P l.
+  Proof. intros. unfold contains. eauto. Qed.
+
+End Contains.
+
+Section Empty.
+
+  Definition al_empty {T:Type} : assoc_list T := nil.
+
+  Theorem empty_invariant : forall (T:Type), al_invariant (@al_empty T).
+  Proof. constructor. Qed.
+
+End Empty.
+
+Section Alter.
+
+  Variable T : Type.
+
+  Let alter_tail (k:N) (v:option T) (t:assoc_list T) :=
+    match v with
+      | None    => t
+      | Some v' => (k,v') :: t
+    end.
+
+  Fixpoint al_alter (f:option T -> option T) (k:N) (l:assoc_list T) : assoc_list T :=
+    match l with
+      | nil    => alter_tail k (f None) nil
+      | h :: t =>
+        let (k',v) := h in
+        if N.eq_dec k' k
+        then alter_tail k (f (Some v)) t
+        else h :: al_alter f k t
+    end.
+  Global Arguments al_alter : default implicits.
+
+  Theorem in_alter_tail :
+    forall (k k':N) (v:T) (x:option T) (l:assoc_list T),
+      In (k,v) l -> In (k,v) (alter_tail k' x l).
+  Proof.
+    Hint Resolve in_eq in_cons.
+    intros k k' v x l. unfold alter_tail. destruct x; auto.
+  Qed.
+
+  Theorem in_alter_tail_inv :
+    forall (k k':N) (v:T) (x:option T) (l:assoc_list T),
+      k <> k' -> In (k,v) (alter_tail k' x l) -> In (k,v) l.
+  Proof.
+    intros k k' v x l ineq. destruct x.
+    - simpl. destruct 1 as [H|H].
+      + inversion H. subst. exfalso. auto.
+      + assumption.
+    - trivial.
+  Qed.
+
+  Theorem in_tail_inv :
+    forall (k k':N) (v v':T) (l:assoc_list T),
+      k <> k' -> In (k,v) ((k',v') :: l) -> In (k,v) l.
+  Proof.
+    intros k k' v v' l ineq.
+    destruct 1 as [H|H].
+    - inversion H. subst. exfalso. auto.
+    - auto.
+  Qed.
+
+  Theorem alter_preserve_other :
+    forall (l:assoc_list T) (k1 k2:N) (f:option T -> option T) (v:T),
+      k1 <> k2 -> (In (k1,v) l <-> In (k1,v) (al_alter f k2 l)).
+  Proof.
+    Hint Resolve in_cons in_eq in_tail_inv in_alter_tail.
+    intros l k1 k2 f v ineq.
+    induction l as [|[k' v'] t IH].
+    - intros. split.
+      + contradiction.
+      + simpl. destruct (f None).
+        * destruct 1 as [H|H]; inversion H; auto.
+        * destruct 1.
+    - split.
+      + intros H. apply in_inv in H. apply proj1 in IH.
+        simpl. destruct (N.eq_dec k' k2).
+        * subst. eauto.
+        * simpl. destruct H; eauto.
+      + simpl. apply proj2 in IH. intros H. destruct (N.eq_dec k' k2).
+        * simpl in H. subst. apply in_alter_tail_inv in H; auto.
+        * simpl. destruct H; eauto.
+  Qed.
+
+  Theorem alter_invariant :
+    forall (l:assoc_list T) (k:N) (f:option T -> option T),
+      al_invariant l -> al_invariant (al_alter f k l).
+  Proof.
+    Hint Constructors al_invariant.
+    Hint Resolve al_invariant_cons not_in_domain_nil.
+    Hint Resolve <- alter_preserve_other.
+    Hint Unfold in_domain.
+    intros l k f inv_l.
+    induction l as [|[k' v'] t IH].
+    - simpl. destruct (f None); simpl; auto.
+    - simpl. inversion inv_l. destruct (N.eq_dec k' k).
+      + subst. destruct (f (Some v')); simpl; auto.
+      + subst. apply al_invariant_cons.
+        * destruct 1 as [v H]. eauto.
+        * eauto.
+  Qed.
+
+End Alter.
+
+Section Remove.
+
+  Variable T : Type.
+
+  Definition al_remove : N -> assoc_list T -> assoc_list T := al_alter (fun _ => None).
+  Global Arguments al_remove : default implicits.
+
+  Theorem remove_empty : forall k, al_remove k al_empty = al_empty.
+  Proof. intros. reflexivity. Qed.
+
+  Theorem remove_not_in :
+    forall (l:assoc_list T) (k:N), al_invariant l -> ~in_domain k (al_remove k l).
+  Proof.
+    Hint Resolve -> in_domain_inv_tail.
+    intros l k inv_l. induction l as [|[k' v'] t IH].
+    - destruct 1. auto.
+    - unfold al_remove. simpl. inversion inv_l. destruct (N.eq_dec k' k).
+      + subst. assumption.
+      + subst. intros H. apply IH; eauto.
+  Qed.
+
+  Theorem remove_subset :
+    forall (l:assoc_list T) (k kr:N) (v:T),
+      al_invariant l -> In (k,v) (al_remove kr l) -> In (k,v) l.
+  Proof.
+    Hint Resolve <- alter_preserve_other.
+    Hint Resolve remove_not_in In_in_domain.
+    intros l k kr v H. destruct (N.eq_dec k kr).
+    - intros. exfalso. subst. eapply remove_not_in; eauto.
+    - eauto.
+  Qed.
+
+  Theorem remove_invariant :
+    forall (l:assoc_list T) (k:N), al_invariant l -> al_invariant (al_remove k l).
+  Proof.
+    Hint Resolve alter_invariant. unfold al_remove. eauto.
+  Qed.
+
+  Theorem remove_preserve_other :
+    forall (l:assoc_list T) (k k':N) (v:T),
+      k <> k' -> (In (k,v) l <-> In (k,v) (al_remove k' l)).
+  Proof.
+    Hint Resolve alter_preserve_other.
+    intros. unfold al_remove. eauto.
+  Qed.
 
 
-Section EmptyTheorems.
+End Remove.
 
-Variable T : Type.
+Section Insert.
 
-Theorem assoc_empty : forall (k:N), assoc k (@empty T) = None.
-Proof. reflexivity. Qed.
+  Variable T : Type.
 
-Theorem empty_invariant : al_invariant T empty.
-Proof. constructor. Qed.
+  Definition al_insert (k:N) (v:T): assoc_list T -> assoc_list T :=
+    al_alter (fun _ => Some v) k.
+  Global Arguments al_insert : default implicits.
 
-End EmptyTheorems.
+  Theorem insert_In :
+    forall (l:assoc_list T) (k:N) (v:T),
+      In (k,v) (al_insert k v l).
+  Proof.
+    Hint Resolve in_eq in_cons.
+    intros l k v. unfold al_insert. induction l as [|[k' v'] t IH].
+    - simpl. eauto.
+    - simpl. destruct (N.eq_dec k' k); eauto.
+  Qed.
 
-Section RemoveTheorems.
+  Theorem insert_in_domain :
+    forall (l:assoc_list T) (k:N) (v:T),
+      in_domain k (al_insert k v l).
+  Proof.
+    Hint Resolve In_in_domain insert_In.
+    eauto.
+  Qed.
 
-Variable T : Type.
+  Theorem insert_domain_superset :
+    forall (l:assoc_list T) (k ki:N) (vi:T),
+      in_domain k l -> in_domain k (al_insert ki vi l).
+  Proof.
+    Hint Resolve In_in_domain insert_in_domain.
+    Hint Resolve -> alter_preserve_other.
+    intros l k ki vi in_l. destruct (N.eq_dec k ki).
+    - subst. eauto.
+    - destruct in_l as [v H]. unfold al_insert. eauto.
+  Qed.
 
-Theorem remove_subset :
-  forall (l:assoc_list T) (k k':N) (P:T -> Prop),
-    contains T k P (remove k' l) -> contains T k P l.
-Proof.
-  Hint Resolve <- contains_inv.
-  intros l k k' P. induction l as [|[k'' v] t IH].
-  - destruct 1 as [v [in_nil HP]]. contradiction.
-  - simpl. destruct (N.eq_dec k'' k').
-    + auto.
-    + rewrite contains_inv. destruct 1; subst; auto.
-Qed.
+  Theorem insert_invariant :
+    forall (l:assoc_list T) (k:N) (v:T),
+      al_invariant l -> al_invariant (al_insert k v l).
+  Proof. Hint Resolve alter_invariant. unfold al_insert. auto. Qed.
 
-Theorem remove_invariant :
-  forall (l:assoc_list T) (k:N), al_invariant T l -> al_invariant T (remove k l).
-Proof.
-  Hint Unfold not in_domain.
-  Hint Resolve remove_subset al_invariant_cons.
-  intros l k. induction l as [|[k' v] t IH].
-  - trivial.
-  - inversion 1. subst. simpl.
-    destruct (N.eq_dec k' k); intuition eauto 6.
-Qed.
+  Theorem insert_preserve_other :
+    forall (l:assoc_list T) (k k':N) (v v':T),
+      k <> k' -> (In (k,v) l <-> In (k,v) (al_insert k' v' l)).
+  Proof. Hint Resolve alter_preserve_other. unfold al_insert. auto. Qed.
 
-Theorem remove_preserve_other :
-  forall (l:assoc_list T) (k k':N) (P:T -> Prop),
-    k' <> k -> contains T k P l -> contains T k P (remove k' l).
-Proof.
-  intros l k k' P ineq. induction l as [|[k'' v] t IH].
-  - trivial.
-  - simpl. rewrite contains_inv. destruct (N.eq_dec k'' k').
-    + subst. tauto.
-    + intuition auto.
-Qed.
+End Insert.
 
-Theorem not_in_remove :
-  forall (l:assoc_list T) (k:N), al_invariant T l -> ~in_domain T k (remove k l).
-Proof.
-  intros l k inv_l. induction l as [|[k' v] t IH].
-  - destruct 1. intuition auto.
-  - simpl. inversion inv_l. subst. destruct (N.eq_dec k' k); subst.
-    + auto.
-    + rewrite in_domain_inv. tauto.
-Qed.
+Section Assoc.
 
-End RemoveTheorems.
+  Variable T : Type.
 
-Section InsertTheorems.
+  Fixpoint al_assoc (k:N) (l:assoc_list T) : option T :=
+    match l with
+      | nil    => None
+      | h :: t => if N.eq_dec (fst h) k then Some (snd h) else al_assoc k t
+    end.
+  Global Arguments al_assoc : default implicits.
 
-Variable T : Type.
-
-Theorem insert_domain_superset :
-  forall (l:assoc_list T) (k k':N) (v:T),
-    in_domain T k l -> in_domain T k (insert k' v l).
-Proof.
-  Hint Resolve <- in_domain_inv.
-  Hint Resolve remove_preserve_other.
-  Hint Unfold in_domain.
-  intros. unfold insert. destruct (N.eq_dec k k'); auto.
-Qed.
-
-Theorem insert_invariant :
-  forall (l:assoc_list T) (k:N) (v:T), al_invariant T l -> al_invariant T (insert k v l).
-Proof.
-  Hint Resolve al_invariant_cons remove_invariant not_in_remove.
-  intros. unfold insert. intuition auto.
-Qed.
-
-Theorem insert_preserve_other :
-  forall (l:assoc_list T) (k k':N) (v:T) (P:T -> Prop),
-    k' <> k -> (contains T k P (insert k' v l) <-> contains T k P l).
-Proof.
-  Hint Resolve remove_subset.
-  intros l k k' v P ineq. unfold insert. rewrite contains_inv. split; intuition eauto.
-Qed.
-
-Theorem contains_insert :
-  forall (l:assoc_list T) (k:N) (v:T) (P:T -> Prop),
-    P v -> contains T k P (insert k v l).
-Proof. intros. unfold insert. apply contains_inv. tauto. Qed.
-
-Theorem in_insert :
-  forall (l:assoc_list T) (k:N) (v:T), in_domain T k (insert k v l).
-Proof. intros. apply contains_insert. apply I. Qed.
-
-End InsertTheorems.
-
-Section AssocTheorems.
-
-Variable T : Type.
-
-Theorem assoc_in_contains :
-  forall (l:assoc_list T) (k:N) (v:T),
-    assoc k l = Some v -> contains T k (eq v) l.
-Proof.
-  Hint Resolve <- contains_inv.
-  intros l k v.
-  induction l as [|[k' v'] t IH].
+  Theorem assoc_In :
+    forall (l:assoc_list T) (k:N) (v:T),
+      al_assoc k l = Some v -> In (k,v) l.
+  Proof.
+    Hint Resolve in_eq in_cons.
+    intros l k v.
+    induction l as [|[k' v'] t IH].
     + discriminate.
     + simpl. destruct (N.eq_dec k' k); inversion 1; subst; auto.
-Qed.
+  Qed.
 
-Theorem contains_assoc_in :
-  forall (l:assoc_list T) (k:N) (v:T),
-    al_invariant T l -> contains T k (eq v) l -> assoc k l = Some v.
-Proof.
-  Hint Resolve contains_in_domain.
-  intros l k v inv_l.
-  - induction l as [|[k' v'] t IH].
-    + destruct 1 as [v' [H HP]]. contradiction.
-    + inversion inv_l. subst. rewrite contains_inv. simpl. destruct (N.eq_dec k' k).
-      * destruct 1 as [[ke ve] | contains_in]; [|exfalso]; subst; eauto.
-      * intuition auto.
-Qed.
+  Theorem In_assoc :
+    forall (l:assoc_list T) (k:N) (v:T),
+      al_invariant l -> In (k,v) l -> al_assoc k l = Some v.
+  Proof.
+    Hint Resolve In_in_domain.
+    intros l k v inv_l. induction l as [|[k' v'] t IH].
+    - contradiction.
+    - inversion inv_l. subst. simpl. destruct (N.eq_dec k' k).
+      + destruct 1 as [E | in_t]; [inversion E|exfalso]; subst; eauto.
+      + destruct 1 as [E | in_t]; [inversion E;exfalso|]; subst; eauto.
+  Qed.
 
-Theorem assoc_in_domain :
-  forall (l:assoc_list T) (k:N),
-    (exists v, assoc k l = Some v) <-> in_domain T k l.
-Proof.
-   Hint Resolve <- in_domain_inv.
-   intros l k. split.
-   - induction l as [|[k' v'] t IH].
-     + destruct 1. discriminate.
-     + simpl. destruct (N.eq_dec k' k); subst; auto.
-   - induction l as [|[k' v'] t IH].
-     + destruct 1. exfalso. intuition auto.
-     + rewrite in_domain_inv. simpl. destruct (N.eq_dec k' k); subst; intuition eauto.
-Qed.
+  Theorem assoc_in_domain :
+    forall (l:assoc_list T) (k:N),
+      ((exists v, al_assoc k l = Some v) <-> in_domain k l).
+  Proof.
+    Hint Resolve In_in_domain assoc_In in_eq in_cons.
+    intros l k. split.
+    - destruct 1; eauto.
+    - intros in_l. induction l as [|[k' v] t IH].
+      + destruct in_l. contradiction.
+      + apply in_domain_inv in in_l. simpl. destruct (N.eq_dec k' k); intuition eauto.
+  Qed.
 
-Theorem assoc_in_1 :
-  forall (l:assoc_list T) (k:N) (v:T),
-    assoc k l = Some v -> in_domain T k l.
-Proof. Hint Resolve -> assoc_in_domain. eauto. Qed.
+  Theorem assoc_in_1 :
+    forall (l:assoc_list T) (k:N) (v:T),
+      al_assoc k l = Some v -> in_domain k l.
+  Proof. Hint Resolve -> assoc_in_domain. eauto. Qed.
 
-Theorem assoc_not_in :
-  forall (l:assoc_list T) (k:N), assoc k l = None <-> ~in_domain T k l.
-Proof.
-  Hint Resolve assoc_in_contains.
-  intros. split.
-  - destruct (assoc k l) eqn:A.
-    + discriminate 1.
-    + intros. rewrite <- assoc_in_domain. rewrite A. destruct 1. discriminate.
-  - destruct (assoc k l) eqn:A.
-    + intros. exfalso. eauto.
-    + reflexivity.
-Qed.
+  Theorem assoc_not_in :
+    forall (l:assoc_list T) (k:N),
+      (al_assoc k l = None <-> ~in_domain k l).
+  Proof.
+    Hint Resolve assoc_In.
+    intros. split.
+    - destruct (al_assoc k l) eqn:A.
+      + discriminate 1.
+      + intros. eauto. rewrite <- assoc_in_domain.
+        rewrite A. destruct 1. discriminate.
+    - destruct (al_assoc k l) eqn:A.
+      + intros. exfalso. eauto.
+      + reflexivity.
+  Qed.
 
-End AssocTheorems.
+End Assoc.
+
+Section InsertMerge.
+
+  Variable T : Type.
+
+  Let alter_fun (f:T -> T) (def:T) (x:option T) : option T :=
+    Some (match x with | None => def | Some v => f v end).
+
+  Definition al_insert_merge (k:N) (f:T -> T) (def:T) : assoc_list T -> assoc_list T :=
+    al_alter (alter_fun f def) k.
+  Global Arguments al_insert_merge : default implicits.
+
+  Theorem insert_merge_inserts :
+    forall (l:assoc_list T) (k:N) (f:T -> T) (def:T),
+      in_domain k (al_insert_merge k f def l).
+  Proof.
+    Hint Resolve <- in_domain_inv.
+    intros l k f def. unfold al_insert_merge. induction l as [|[k' v'] t IH].
+    - simpl. auto.
+    - simpl. destruct (N.eq_dec k' k); auto.
+  Qed.
+
+  Theorem insert_merge_superset :
+    forall (l:assoc_list T) (k k':N) (f:T -> T) (def:T),
+      in_domain k l -> in_domain k (al_insert_merge k' f def l).
+  Proof.
+    Hint Resolve insert_merge_inserts.
+    Hint Resolve -> alter_preserve_other.
+    Hint Unfold in_domain.
+    intros l k k' f def H.
+    destruct (N.eq_dec k k').
+    - subst. eauto.
+    - unfold al_insert_merge. destruct H. eauto.
+  Qed.
+
+  Theorem insert_merge_preserve_other :
+    forall (l:assoc_list T) (k k':N) (v:T) (f:T -> T) (def:T),
+      k <> k' -> (In (k,v) l <-> In (k,v) (al_insert_merge k' f def l)).
+  Proof.
+    Hint Resolve alter_preserve_other.
+    unfold al_insert_merge. auto.
+  Qed.
+
+  Theorem In_insert_merge_inv :
+    forall (l:assoc_list T) (k:N) (v def:T) (f:T -> T),
+      al_invariant l ->
+      In (k,v) (al_insert_merge k f def l) ->
+      (~in_domain k l /\ v = def) \/ (contains k (fun x => f x = v) l).
+  Proof.
+    Hint Resolve not_in_domain_nil in_eq in_cons In_in_domain not_in_domain_cons.
+    Hint Resolve In_contains in_cons_inv.
+    intros l k v def f inv_l H. induction l as [|[k' v'] t IH].
+    - destruct H as [E|E]; inversion E; subst; eauto.
+    - unfold al_insert_merge in H. simpl in H. inversion inv_l. subst.
+      destruct (N.eq_dec k' k).
+      + apply in_eq_inv in H; subst; eauto.
+      + destruct IH as [[? ?]|[? [? ?]]]; eauto.
+  Qed.
+
+  Theorem insert_merge_invariant :
+    forall (l:assoc_list T) (k:N) (f:T -> T) (def:T),
+      al_invariant l -> al_invariant (al_insert_merge k f def l).
+  Proof. Hint Resolve alter_invariant. unfold al_insert_merge. auto. Qed.
+
+  Theorem insert_merge_contains :
+    forall (l:assoc_list T) (k:N) (f:T -> T) (def:T) (P:T -> Prop),
+      (~in_domain k l -> P def) ->
+      (forall v, In (k,v) l -> P (f v)) -> contains k P (al_insert_merge k f def l).
+  Proof.
+    Hint Resolve in_eq in_cons In_contains not_in_domain_nil.
+    Hint Resolve -> in_domain_inv_tail.
+    intros l k f def P Pdef Pf.
+    unfold al_insert_merge. induction l as [|[k' v'] t IH].
+    - simpl. eauto.
+    - simpl. destruct (N.eq_dec k' k).
+      + subst. eauto.
+      + destruct IH as [v [H Q]]; eauto.
+  Qed.
+
+End InsertMerge.
 
 Section Merge.
 
-Variable T : Type.
+  Variable T : Type.
 
-Fixpoint merge (f:T -> T -> T) (l1:assoc_list T) (l2:assoc_list T) : assoc_list T :=
-  match l1 with
-    | nil        => l2
-    | (k,v1) :: l1_t =>
-      match assoc k l2 with
-        | None    => (k,v1) :: merge f l1_t l2
-        | Some v2 => (k,f v1 v2) :: merge f l1_t (remove k l2)
-      end
-  end.
-Global Arguments merge : default implicits.
+  Fixpoint al_merge (f:T -> T -> T) (l1:assoc_list T) (l2:assoc_list T) : assoc_list T :=
+    match l1 with
+      | nil            => l2
+      | (k,v1) :: l1_t => al_insert_merge k (f v1) v1 (al_merge f l1_t l2)
+    end.
+  Global Arguments al_merge : default implicits.
 
-Definition union : assoc_list T -> assoc_list T -> assoc_list T :=
-  merge (fun _ b => b).
-Global Arguments union : default implicits.
+  Definition al_union : assoc_list T -> assoc_list T -> assoc_list T :=
+    al_merge (fun _ b => b).
+  Global Arguments al_union : default implicits.
 
-Theorem merge_no_new_elements :
-  forall (l1 l2:assoc_list T) (f:T -> T -> T) (k:N),
-    ~in_domain T k l1 -> ~in_domain T k l2 -> ~in_domain T k (merge f l1 l2).
-Proof.
-  Hint Unfold not in_domain.
-  Hint Resolve remove_subset.
-  intros l1 l2 f k H.
-  generalize dependent l2.
-  induction l1 as [|[k' v] t IH].
-  - intros. assumption.
-  - simpl. intros l2. rewrite in_domain_inv in H.
-    destruct (assoc k' l2) eqn:A; rewrite in_domain_inv; intuition eauto.
-Qed.
+  Theorem merge_no_new_elements :
+    forall (l1 l2:assoc_list T) (f:T -> T -> T) (k:N),
+      ~in_domain k l1 -> ~in_domain k l2 -> ~in_domain k (al_merge f l1 l2).
+  Proof.
+    Hint Unfold in_domain.
+    Hint Resolve <- insert_merge_preserve_other in_domain_inv.
+    intros l1 l2 f k H.
+    induction l1 as [|[k' v] t IH].
+    - intros. assumption.
+    - simpl. intros not_in_l2.
+      intros R. unfold not in H. destruct R.
+      destruct (N.eq_dec k k').
+      + subst. eauto.
+      + apply IH; eauto.
+  Qed.
 
-Theorem merge_invariant :
-  forall (l1 l2:assoc_list T) (f:T -> T -> T),
-    al_invariant T l1 -> al_invariant T l2 -> al_invariant T (merge f l1 l2).
-Proof.
-  Hint Resolve al_invariant_cons merge_no_new_elements not_in_remove remove_invariant.
-  Hint Resolve -> assoc_not_in assoc_in_domain.
-  intros l1 l2 f inv_l1.
-  generalize dependent l2.
-  induction l1 as [|[k v] t IH].
-  - intros. assumption.
-  - intros l2 inv_l2. inversion inv_l1. subst. simpl. case_eq (assoc k l2); auto.
-Qed.
+  Theorem merge_invariant :
+    forall (l1 l2:assoc_list T) (f:T -> T -> T),
+      al_invariant l1 -> al_invariant l2 -> al_invariant (al_merge f l1 l2).
+  Proof.
+    Hint Resolve insert_merge_invariant.
+    intros l1 l2 f inv_l1 inv_l2.
+    induction l1 as [|[k v] t IH].
+    - assumption.
+    - inversion inv_l1. simpl. eauto.
+  Qed.
 
-Theorem merge_superset_first :
-  forall (l1 l2:assoc_list T) (f:T -> T -> T) (k:N),
-    in_domain T k l1 -> in_domain T k (merge f l1 l2).
-Proof.
-  Hint Resolve <- in_domain_inv.
-  Hint Resolve remove_subset.
-  intros l1 l2 f k.
-  generalize dependent l2.
-  - induction l1 as [|[k' v] t IH].
-    + destruct 1. exfalso. intuition auto.
-    + intros l2. rewrite in_domain_inv. simpl.
-      destruct (assoc k' l2) eqn:A; intuition auto.
-Qed.
+  Theorem merge_superset_first :
+    forall (l1 l2:assoc_list T) (f:T -> T -> T) (k:N),
+      in_domain k l1 -> in_domain k (al_merge f l1 l2).
+  Proof.
+    Hint Resolve insert_merge_superset insert_merge_inserts.
+    intros l1 l2 f k in_l1.
+    - induction l1 as [|[k' v] t IH].
+      + simpl. exfalso. eapply not_in_domain_nil. eauto.
+      + simpl. apply in_domain_inv in in_l1. destruct in_l1; subst; eauto.
+  Qed.
 
-Theorem merge_superset_second :
-  forall (l1 l2:assoc_list T) (f:T -> T -> T) (k:N),
-    in_domain T k l2 -> in_domain T k (merge f l1 l2).
-Proof.
-  Hint Resolve <- contains_inv.
-  Hint Resolve remove_preserve_other.
-  intros l1 l2 f k.
-  generalize dependent l2.
-  - unfold in_domain. induction l1 as [|[k' v] t IH].
-    + trivial.
-    + intros l2. intros H. simpl.
-      destruct (assoc k' l2) eqn:A; destruct (N.eq_dec k' k); subst; auto.
-Qed.
+  Theorem merge_superset_second :
+    forall (l1 l2:assoc_list T) (f:T -> T -> T) (k:N),
+      in_domain k l2 -> in_domain k (al_merge f l1 l2).
+  Proof.
+    Hint Resolve insert_merge_superset insert_merge_inserts.
+    intros l1 l2 f k in_l2.
+    - induction l1 as [|[k' v] t IH].
+      + trivial.
+      + simpl. eauto.
+  Qed.
 
 End Merge.
 
-Section RevAssoc.
-
-Variable T : Type.
-
-Fixpoint rev_assoc (p:T -> bool) (l:assoc_list T) : list N :=
-  match l with
-    | nil         => nil
-    | (k,v) :: t => if p v then k :: rev_assoc p t else rev_assoc p t
-  end.
-Global Arguments rev_assoc : default implicits.
-
-Theorem rev_assoc_assoc :
-  forall (f:T -> bool) (l:assoc_list T) (k:N),
-    al_invariant T l ->
-    In k (rev_assoc f l) -> contains T k (fun v => f v = true) l.
-Proof.
-  intros f l k inv_l H. induction l as [|[k' v'] t IH].
-  - contradiction.
-  - apply contains_inv. simpl in H. inversion inv_l. subst. destruct (f v') eqn:fv.
-    + apply in_inv in H. destruct (N.eq_dec k' k); intuition eauto.
-    + destruct (N.eq_dec k' k). subst.
-      * Hint Resolve contains_in_domain. exfalso. intuition eauto.
-      * eauto.
-Qed.
-
-Theorem assoc_rev_assoc :
-  forall (f:T -> bool) (l:assoc_list T) (k:N),
-    al_invariant T l ->
-    contains T k (fun v => f v = true) l -> In k (rev_assoc f l).
-Proof.
-  Hint Unfold contains.
-  Hint Resolve in_eq in_cons.
-  intros f l k inv_l. induction l as [|[k' v'] t IH].
-  - destruct 1 as [v [a fv]]. auto.
-  - simpl. inversion inv_l. subst. destruct 1 as [v [v_in fvt]].
-    apply in_inv in v_in. destruct v_in as [eq|in_t].
-    + inversion eq. subst. rewrite fvt. auto.
-    + destruct (f v') eqn:fv'; eauto 6.
-Qed.
-
-End RevAssoc.
-
 Section Filter.
 
-Variable T : Type.
+  Variable T : Type.
 
-Definition al_filter (f:N -> T -> bool) : assoc_list T -> assoc_list T :=
-  filter (fun x => match x with (k,v) => f k v end).
-Global Arguments al_filter : default implicits.
+  Definition al_filter (f:N -> T -> bool) : assoc_list T -> assoc_list T :=
+    filter (fun x => match x with (k,v) => f k v end).
+  Global Arguments al_filter : default implicits.
 
-Theorem al_filter_subset :
-  forall (l:assoc_list T) (k:N) (P:T -> Prop) (f:N -> T -> bool),
-    contains T k P (al_filter f l) -> contains T k P l.
-Proof.
-  Hint Resolve <- contains_inv.
-  intros l k P f. induction l as [|[k' v] t IH].
-  - auto.
-  - simpl. destruct (f k' v) eqn:fkv.
-    + rewrite contains_inv. destruct 1 as [[ke Pv] | contains_filter_t]; auto.
-    + auto.
-Qed.
+  Theorem filter_subset :
+    forall (l:assoc_list T) (k:N) (v:T) (f:N -> T -> bool),
+      In (k,v) (al_filter f l) -> In (k,v) l.
+  Proof.
+    intros l k P f. induction l as [|[k' v] t IH].
+    - auto.
+    - simpl. destruct (f k' v) eqn:fkv.
+      + simpl. destruct 1 as [E|in_t]; [inversion E|]; subst; eauto.
+      + eauto.
+  Qed.
 
-Theorem al_filter_invariant :
-  forall (l:assoc_list T) (f:N -> T -> bool),
-    al_invariant T l -> al_invariant T (al_filter f l).
-Proof.
-  Hint Resolve al_filter_subset al_invariant_cons.
-  Hint Unfold in_domain.
-  intros l f H. induction l as [|[k v] t IH].
-  - auto.
-  - simpl. inversion H; subst. destruct (f k v) eqn:fkv; eauto 7.
-Qed.
+  Theorem filter_predicate_true :
+    forall (l:assoc_list T) (k:N) (v:T) (f:N -> T -> bool),
+      In (k,v) (al_filter f l) -> f k v = true.
+  Proof.
+    unfold al_filter. intros l k v f. rewrite filter_In. tauto.
+  Qed.
+
+  Theorem filter_invariant :
+    forall (l:assoc_list T) (f:N -> T -> bool),
+      al_invariant l -> al_invariant (al_filter f l).
+  Proof.
+    Hint Resolve filter_subset al_invariant_cons.
+    Hint Resolve <- in_domain_inv.
+    Hint Unfold in_domain.
+    intros l f H. induction l as [|[k v] t IH].
+    - auto.
+    - simpl. inversion H as [|k' v' t' not_in_t inv_t]. subst. destruct (f k v) eqn:fkv.
+      + apply al_invariant_cons; try (destruct 1); eauto.
+      + auto.
+  Qed.
 
 End Filter.
 
-Definition update {T:Type} (k:N) (f:T -> T) (l:assoc_list T) : assoc_list T :=
-  match assoc k l with
-    | None   => l
-    | Some v => insert k v l
-  end.
+Section RevAssoc.
 
-Definition insert_merge {T:Type} (k:N) (f:T -> T) (def:T) (l:assoc_list T) : 
-  assoc_list T :=
-  insert k (f (match assoc k l with
-                 | None   => def
-                 | Some v => v
-               end)) l.
+  Variable T : Type.
 
-Definition al_map {A B:Type} (f:N -> A -> B) : assoc_list A -> assoc_list B :=
-  map (fun x => match x with (k,v) => (k,f k v) end).
+  Definition al_rev_assoc (p:T -> bool) (l:assoc_list T) : list N :=
+    map (@fst N T) (al_filter (fun _ => p) l).
+  Global Arguments al_rev_assoc : default implicits.
+
+  Let map_fst_In :
+    forall (k:N) (l:assoc_list T), In k (map (@fst N T) l) -> exists v, In (k,v) l.
+  Proof.
+    intros k l H. induction l as [|[k' v'] t IH].
+    - contradiction.
+    - simpl. destruct H.
+      + subst. eauto.
+      + destruct IH; eauto.
+  Qed.
+
+  Theorem rev_assoc_assoc :
+    forall (f:T -> bool) (l:assoc_list T) (k:N),
+      In k (al_rev_assoc f l) -> exists v, In (k,v) l /\ f v = true.
+  Proof.
+    Hint Resolve filter_subset.
+    unfold al_rev_assoc. intros f l k H.
+    apply map_fst_In in H. destruct H as [v H]. exists v. split.
+    + eauto.
+    + apply filter_predicate_true in H. eauto.
+  Qed.
+
+  Theorem assoc_rev_assoc :
+    forall (f:T -> bool) (l:assoc_list T) (k:N) (v:T),
+      al_invariant l ->
+      In (k,v) l -> f v = true -> In k (al_rev_assoc f l).
+  Proof.
+    Hint Resolve in_eq in_cons.
+    intros f l k v inv_l. induction l as [|[k' v'] t IH].
+    - contradiction.
+    - simpl. inversion inv_l. subst. destruct 1 as [eq|in_t].
+      + inversion eq. subst. intros fvt. unfold al_rev_assoc. simpl. rewrite fvt. simpl.
+        eauto.
+      + unfold al_rev_assoc. simpl. destruct (f v') eqn:fv'; simpl; eauto.
+  Qed.
+
+End RevAssoc.
+
+Section Update.
+
+  Variable T : Type.
+
+  Let alter_fun (f:T -> T) (x:option T) : option T :=
+    match x with | None => None | Some v => Some (f v) end.
+
+  Definition al_update (k:N) (f:T -> T) : assoc_list T -> assoc_list T :=
+    al_alter (alter_fun f) k.
+  Global Arguments al_update : default implicits.
+
+  Theorem update_invariant :
+    forall (l:assoc_list T) (k:N) (f:T -> T),
+      al_invariant l -> al_invariant (al_update k f l).
+  Proof. Hint Resolve alter_invariant. unfold al_update. auto. Qed.
+
+  Theorem update_updates :
+    forall (l:assoc_list T) (k:N) (v:T) (f:T -> T),
+      al_invariant l -> (In (k,v) l -> In (k,f v) (al_update k f l)).
+  Proof.
+    Hint Resolve in_eq in_cons In_in_domain.
+    intros l k v f inv_l.
+    induction l as [|[k'' v''] t IH].
+    - contradiction.
+    - unfold al_update. simpl. inversion inv_l. destruct (N.eq_dec k'' k).
+      + destruct 1 as [E|E]; [inversion E|exfalso]; subst; eauto.
+      + simpl. destruct 1 as [E|E]; [inversion E;exfalso|]; subst; eauto.
+  Qed.
+
+  Theorem update_preserve_at_k :
+    forall (l:assoc_list T) (k:N) (f:T -> T),
+      in_domain k l <-> in_domain k (al_update k f l).
+  Proof.
+    intros l k f. induction l as [|[k' v'] t IH].
+    - split; destruct 1; contradiction.
+    - unfold al_update. simpl. destruct (N.eq_dec k' k).
+      + subst. split; eauto.
+      + rewrite_all in_domain_inv_tail; eauto.
+  Qed.
+
+  Theorem update_preserve_domain :
+    forall (l:assoc_list T) (k k':N) (f:T -> T),
+      in_domain k l <-> in_domain k (al_update k' f l).
+  Proof.
+    Hint Resolve update_preserve_at_k.
+    Hint Resolve -> alter_preserve_other.
+    Hint Resolve <- alter_preserve_other.
+    intros l k k' f. destruct (N.eq_dec k k').
+    - subst. eauto.
+    - unfold al_update; split; destruct 1; eauto.
+  Qed.
+
+  Theorem update_preserve_other :
+    forall (l:assoc_list T) (f:T -> T) (k k':N) (v:T),
+      k <> k' -> (In (k,v) l <-> In (k,v) (al_update k' f l)).
+  Proof.
+    Hint Resolve alter_preserve_other.
+    intros. unfold al_update. eauto.
+  Qed.
+
+  Theorem In_update_inv :
+    forall (l:assoc_list T) (f:T -> T) (k:N) (v:T),
+      al_invariant l -> (In (k,v) (al_update k f l) <-> exists x, In (k,x) l /\ f x = v).
+  Proof.
+    Hint Resolve In_in_domain update_updates in_cons_inv.
+    intros l f k v inv_l. split.
+    - unfold al_update. induction l as [|[k' v'] t IH].
+      + simpl. contradiction.
+      + simpl. inversion inv_l. subst. intros H. destruct (N.eq_dec k' k).
+        * apply in_eq_inv in H; subst; eauto.
+        * destruct IH as [? [? ?]]; eauto.
+    - destruct 1 as [? [? ?]]. subst. auto.
+  Qed.
+
+End Update.
+
+Section Map.
+
+  Variable A B : Type.
+
+  Let map_fun (f:N -> A -> B) (x:N * A) : (N * B) :=
+    match x with (k,v) => (k, f k v) end.
+
+  Definition al_map (f:N -> A -> B) : assoc_list A -> assoc_list B :=
+    map (map_fun f).
+  Global Arguments al_map : default implicits.
+
+  Theorem map_updates_all :
+    forall (l:assoc_list A) (f:N -> A -> B) (k:N) (v:A),
+      In (k,v) l -> In (k,f k v) (al_map f l).
+  Proof.
+    intros l f k v. unfold al_map.
+    replace (k, f k v) with (map_fun f (k,v)) by reflexivity.
+    apply in_map.
+  Qed.
+
+  Theorem map_preserve_domain :
+    forall (l:assoc_list A) (f:N -> A -> B) (k:N),
+      in_domain k l <-> in_domain k (al_map f l).
+  Proof.
+    Hint Resolve In_in_domain map_updates_all.
+    split.
+    - destruct 1. eauto.
+    - unfold al_map. intros H. destruct H as [v H]. apply in_map_iff in H.
+      destruct H as [[k' v'] [H Q]]. inversion H. subst. eauto.
+  Qed.
+
+  Theorem map_invariant :
+    forall (l:assoc_list A) (f:N -> A -> B),
+      al_invariant l -> al_invariant (al_map f l).
+  Proof.
+    Hint Constructors al_invariant.
+    Hint Resolve al_invariant_cons.
+    Hint Resolve <- map_preserve_domain.
+    intros l f inv_l. induction l as [|[k v] t IH].
+    - simpl. auto.
+    - simpl. inversion inv_l. subst. apply al_invariant_cons; eauto.
+  Qed.
+
+End Map.
