MappingDB.v
@@ -1,104 +1,272 @@
 Require Import NArith.
 Require Import List.
 Require Import AssocList.
+Require Import Bool.
 
 Section MappingDB.
-
 Variable kernel_object : Type.
 
-Definition mapping_db : Type := assoc_list (assoc_list kernel_object).
+Section Def.
 
-Definition has_mapping (pd:N) (sel:N) (ko:kernel_object) : mapping_db -> Prop :=
-  contains _ pd (contains _ sel (eq ko)).
+  Definition mapping_db : Type := assoc_list (assoc_list kernel_object).
 
-Definition create_mapping (pd:N) (sel:N) (ko:kernel_object) : mapping_db -> mapping_db :=
-  insert_merge pd (insert sel ko) empty.
+  Definition has_mapping (pd:N) (sel:N) (ko:kernel_object) : mapping_db -> Prop :=
+    contains pd (In (sel,ko)).
 
-Definition remove_mapping (pd:N) (sel:N) : mapping_db -> mapping_db :=
-  update pd (remove sel).
+  Definition in_mapping_db (pd:N) (sel:N) : mapping_db -> Prop :=
+    contains pd (in_domain sel).
 
-Fixpoint restrict (exceptions:assoc_list (list N)) : mapping_db -> mapping_db :=
-  al_map (fun pd mappings =>
-    match assoc pd exceptions with
-      | None     => mappings
-      | Some exc =>
-        al_filter (fun sel _ => if in_dec N.eq_dec sel exc then true else false) mappings
-    end).
+End Def.
 
+Section Create.
 
-Definition remove_all (f:kernel_object -> bool) : mapping_db -> mapping_db :=
-  al_map (fun _ => al_filter (fun _ => f)).
+  Definition create_mapping (pd:N) (sel:N) (ko:kernel_object) :
+    mapping_db -> mapping_db :=
+    al_insert_merge pd (al_insert sel ko) (al_insert sel ko al_empty).
 
-Definition remove_all_except
-           (f:kernel_object -> bool)
-           (exceptions:assoc_list (list N))
-           (db:mapping_db) : mapping_db :=
-  union (restrict exceptions db) (remove_all f db).
+  Theorem create_has_mapping :
+    forall (db:mapping_db) (pd:N) (sel:N) (ko:kernel_object),
+      has_mapping pd sel ko (create_mapping pd sel ko db).
+  Proof.
+    Hint Resolve insert_In In_contains.
+    intros db pd sel ko. unfold has_mapping. unfold create_mapping.
+    apply insert_merge_contains; simpl; eauto.
+  Qed.
 
-Theorem create_preserve_other :
-  forall (db:mapping_db) (pd pd':N) (sel sel':N) (ko ko':kernel_object),
-    (pd' <> pd \/ sel' <> sel) -> al_invariant _ db ->
-    (has_mapping pd sel ko db
-     <-> has_mapping pd sel ko (create_mapping pd' sel' ko' db)).
-Proof.
-  Hint Resolve <- insert_preserve_other.
-  Hint Resolve contains_insert.
-  intros db pd pd' sel sel' ko ko' ineq inv_db. split.
-  - unfold create_mapping. unfold insert_merge. destruct (assoc pd' db) eqn:A.
-    + intros H. unfold has_mapping. destruct (N.eq_dec pd' pd); subst; eauto.
-      destruct ineq as [pde | sele].
-      * eauto.
-      * apply contains_insert. apply insert_preserve_other. assumption. unfold has_mapping in H. apply assoc_in_contains in A.
-        apply contains_combine with (P1 := eq a) in H.
-        unfold contains in H. destruct H as [v [in_db [av E]]].
-        unfold contains. subst. assumption. assumption. assumption.
-    + destruct (N.eq_dec pd' pd). 
-      * destruct ineq as [H|H]; try tauto. subst. unfold has_mapping. intros P. 
-        apply contains_in_domain in P. apply assoc_not_in in A. contradiction.
-      * intros. unfold has_mapping. apply insert_preserve_other. assumption.
-        assumption.
-  - unfold create_mapping. unfold insert_merge. intros H. unfold has_mapping.
-    destruct (assoc pd' db) eqn:A.
-    + destruct ineq as [ineq|ineq]. 
-      * apply insert_preserve_other in H; assumption.
-      * destruct (N.eq_dec pd' pd).
-        subst. unfold has_mapping in H.
-Abort.
+  Lemma ineq_2_dec :
+    forall (a a' b b':N), (a <> a' \/ b <> b') -> (a <> a' \/ (a = a' /\ b <> b')).
+  Proof.
+    intros a a' b b' H. destruct (N.eq_dec a a'); tauto.
+  Qed.
 
-Theorem create_has_mapping :
-  forall (db:mapping_db) (pd:N) (sel:N) (ko:kernel_object),
-    has_mapping pd sel ko (create_mapping pd sel ko db).
-Proof.
-Abort.
+  Theorem create_preserve_other :
+    forall (db:mapping_db) (pd pd':N) (sel sel':N) (ko ko':kernel_object),
+      (pd' <> pd \/ sel' <> sel) -> al_invariant db ->
+      (has_mapping pd sel ko db
+       <-> has_mapping pd sel ko (create_mapping pd' sel' ko' db)).
+  Proof.
+    Hint Resolve <- insert_preserve_other insert_merge_preserve_other.
+    Hint Resolve -> insert_preserve_other insert_merge_preserve_other.
+    Hint Resolve insert_In In_contains In_in_domain al_invariant_in_eq.
+    intros db pd pd' sel sel' ko ko' ineq inv_db. apply ineq_2_dec in ineq.
+    unfold has_mapping. unfold create_mapping. destruct ineq as [H|[? H]].
+    - split;
+      destruct 1 as [pd_mappings [in_db in_pd]];
+      eapply insert_merge_preserve_other in in_db; eauto.
+    - subst. split.
+      + destruct 1 as [pd_mappings [in_db in_pd]]. apply insert_merge_contains.
+        * intros. exfalso. eauto.
+        * intros. replace v with pd_mappings by eauto. eauto.
+      + destruct 1 as [pd_mappings [in_created in_pd]].
+        apply In_insert_merge_inv in in_created as [[? ?] | [? [? ?]]];
+          subst;
+          try (apply insert_preserve_other in in_pd);
+          eauto.
+  Qed.
 
-Theorem remove_removes_mapping :
-  forall (db:mapping_db) (pd:N) (sel:N) (ko:kernel_object),
-    ~has_mapping pd sel ko (remove_mapping pd sel db).
-Proof.
-Abort.
+End Create.
 
-Theorem remove_preserve_other :
-  forall (db:mapping_db) (pd pd':N) (sel sel':N) (ko:kernel_object),
-    (pd' <> pd /\ sel <> sel') ->
-    (has_mapping pd sel ko db <-> has_mapping pd sel ko (remove_mapping pd sel db)).
-Proof.
-Abort.
+Section Delete.
 
-Theorem remove_all_except_removes :
+  Definition delete_mapping (pd:N) (sel:N) : mapping_db -> mapping_db :=
+    al_update pd (al_remove sel).
+
+  Theorem delete_deletes_mapping :
+    forall (db:mapping_db) (pd:N) (sel:N) (ko:kernel_object),
+      (forall k x, In (k,x) db -> al_invariant x) ->
+      al_invariant db -> ~has_mapping pd sel ko (delete_mapping pd sel db).
+  Proof.
+    Hint Unfold not.
+    Hint Resolve remove_not_in In_in_domain.
+    intros db pd sel ko inv inv_l. unfold delete_mapping. unfold has_mapping.
+    destruct 1 as [pdv [pd_in sel_in]].
+    apply In_update_inv in pd_in as [x [in_db rm_eq]];
+      try (eapply remove_not_in with (l := x));
+      subst; eauto.
+  Qed.
+
+  Theorem delete_preserve_other :
+    forall (db:mapping_db) (pd pd':N) (sel sel':N) (ko:kernel_object),
+      al_invariant db ->
+      (forall k x, In (k,x) db -> al_invariant x) ->
+      (pd' <> pd \/ sel <> sel') ->
+      (has_mapping pd sel ko db <-> has_mapping pd sel ko (delete_mapping pd' sel' db)).
+  Proof.
+    Hint Resolve -> update_preserve_other remove_preserve_other.
+    Hint Resolve <- update_preserve_other remove_preserve_other.
+    Hint Resolve update_updates.
+    intros db pd pd' sel sel' ko inv_db inv_all ineq. apply ineq_2_dec in ineq.
+    unfold has_mapping. unfold contains. unfold delete_mapping.
+    destruct ineq as [H|[pd_eq sel_ineq]].
+    - split; destruct 1; intuition eauto.
+    - subst. split; destruct 1 as [pdm [in_db in_pdm]].
+      + eauto.
+      + apply In_update_inv in in_db as [? [? ?]]; subst; eauto.
+  Qed.
+
+End Delete.
+
+Section Union.
+
+  Definition db_union : mapping_db -> mapping_db -> mapping_db :=
+    al_merge (@al_union _).
+
+  Theorem merge_In_first :
+    forall (T:Type) (l1 l2:assoc_list T) (f:T -> T -> T) (v:T) (k:N),
+      al_invariant l1 -> al_invariant l2 -> ~in_domain k l2 -> In (k,v) (al_merge f l1 l2) -> In (k,v) l1.
+  Proof.
+    Hint Resolve In_in_domain in_eq in_cons merge_invariant.
+    Hint Resolve <- insert_merge_preserve_other.
+    intros T l1 l2 f v k inv_l1 inv_l2 not_in_l1 in_merge.
+    induction l1 as [|[k' v'] t IH].
+    - exfalso. eauto.
+    - simpl in in_merge. inversion inv_l1. subst. destruct (N.eq_dec k k').
+      + subst k'. apply In_insert_merge_inv in in_merge as [[_ ve]|contains_merge].
+        * subst. eauto.
+        * destruct contains_merge as [x [x_in _]]. exfalso.
+          eapply merge_no_new_elements with (l1 := t) (l2 := l2); eauto.
+        * eauto.
+      + apply insert_merge_preserve_other in in_merge; eauto.
+  Qed.
+
+  Theorem merge_In_second :
+    forall (T:Type) (l1 l2:assoc_list T) (f:T -> T -> T) (v:T) (k:N),
+      ~in_domain k l1 -> In (k,v) (al_merge f l1 l2) -> In (k,v) l2.
+  Proof.
+    intros T l1 l2 f v k not_in_l2 in_merge.
+    induction l1 as [|[k' v'] t IH].
+    - assumption.
+    - simpl in in_merge. apply not_in_domain_inv in not_in_l2 as [ineq_k not_in_t].
+      apply insert_merge_preserve_other in in_merge; eauto.
+  Qed.
+
+  Theorem merge_In_both :
+    forall (T:Type) (l1 l2:assoc_list T) (f:T -> T -> T) (v:T) (k:N),
+      al_invariant l1 -> al_invariant l2 ->
+      in_domain k l1 -> in_domain k l2 -> In (k,v) (al_merge f l1 l2) ->
+      exists x y, f x y = v /\ In (k,x) l1 /\ In (k,y) l2.
+  Proof.
+    Hint Resolve merge_superset_second merge_invariant In_in_domain in_cons.
+    Hint Resolve -> insert_merge_preserve_other.
+    intros T l1 l2 f v k inv_l1 inv_l2 in_l1 in_l2 in_merge.
+    induction l1 as [|[k' v'] t IH].
+    - destruct in_l1. contradiction.
+    - destruct in_l1 as [x [E | in_t]].
+      + inversion E. subst k'. subst x. clear E.
+        simpl in in_merge. apply In_insert_merge_inv in in_merge.
+        * destruct in_merge as [[not_in_merge ve]|contains_t].
+          { exfalso. eauto. }
+          { unfold contains in contains_t.
+            destruct contains_t as [a [in_merge fe]].
+            clear IH. exists v'. exists a.
+            inversion inv_l1. subst. apply merge_In_second in in_merge;
+              repeat split; auto. }
+        * inversion inv_l1. subst. auto.
+      + inversion inv_l1. subst. simpl in in_merge.
+        destruct (N.eq_dec k k').
+        * subst. exfalso. eauto.
+        * destruct IH as [x' [y' [fe' [in_t' in_l2']]]]; subst; repeat eexists; eauto.
+  Qed.
+
+  Theorem db_union_In_second :
+    forall (db1 db2:mapping_db) (ko:kernel_object) (pd sel:N),
+      al_invariant db1 -> al_invariant db2 ->
+      ~in_mapping_db pd sel db1 -> has_mapping pd sel ko (db_union db1 db2) ->
+      has_mapping pd sel ko db2.
+  Proof.
+    Hint Unfold contains.
+    Hint Resolve In_in_domain.
+    unfold has_mapping. unfold db_union. unfold contains.
+    intros db1 db2 ko pd sel inv_db1 inv_db2 not_in_db1 in_union.
+    destruct in_union as [pdm [in_union in_pdm]].
+    destruct (in_domain_dec _ db1 pd) as [pd_in_db1|pd_not_in_db1].
+    - destruct (in_domain_dec _ db2 pd) as [pd_in_db2|pd_not_in_db2].
+      + apply merge_In_both with (1 := inv_db1) (2 := inv_db2) (3 := pd_in_db1) (4 := pd_in_db2) in in_union.
+        destruct in_union as [x [y [pdme [in_db1 in_db2]]]].
+          subst pdm. destruct (in_domain_dec _ x sel).
+          { exfalso. apply not_in_db1. unfold in_mapping_db. unfold contains. eauto. }
+          { apply merge_In_second in in_pdm; try (eexists; split); eauto. }
+      + apply merge_In_first with (1 := inv_db1) (2 := inv_db2) (3 := pd_not_in_db2) in in_union. exfalso. apply not_in_db1. unfold in_mapping_db. eauto.
+    - apply merge_In_second with (1 := pd_not_in_db1) in in_union.
+      eauto.
+  Qed.
+
+End Union.
+
+Section DeleteAll.
+
+  Definition delete_all_except
+             (f:kernel_object -> bool)
+             (exceptions:assoc_list (list N))
+             : mapping_db -> mapping_db :=
+    al_map
+      (fun pd pdm =>
+         match al_assoc pd exceptions with
+           | None     => al_filter (fun _ x => negb (f x)) pdm
+           | Some exc => al_filter
+                           (fun sel x => negb (andb
+                                                 (f x)
+                                                 (negb (existsb (N.eqb sel) exc))))
+                           pdm
+         end).
+
+  Theorem In_map_iff :
+    forall (A B:Type) (f:N -> A -> B) (l:assoc_list A) (b:B) (k:N),
+      In (k, b) (al_map f l) <-> exists a : A, b = f k a /\ In (k,a) l.
+  Proof.
+    intros A B f l b k. unfold al_map. rewrite in_map_iff. split.
+    - destruct 1 as [x [E H]]. destruct x. inversion E. subst. eauto.
+    - destruct 1 as [a [E H]]. exists (k,a). subst. auto.
+  Qed.
+
+  Theorem al_filter_In :
+    forall (T:Type) (f:N -> T -> bool) (l:assoc_list T) (k:N) (v:T),
+      (f k v = true /\ In (k,v) l) <-> In (k,v) (al_filter f l).
+  Proof.
+    intros. unfold al_filter. rewrite filter_In. tauto.
+  Qed.
+
+  Theorem delete_all_except_deletes :
+    forall (db:mapping_db) (pd:N) (sel:N) (ko:kernel_object) (f:kernel_object -> bool)
+           (exceptions:assoc_list (list N)),
+      has_mapping pd sel ko (delete_all_except f exceptions db) ->
+      f ko = false \/ contains pd (In sel) exceptions.
+  Proof.
+    Hint Resolve assoc_In.
+    intros db pd sel ko f exceptions. unfold has_mapping.
+    unfold delete_all_except. unfold contains. destruct 1 as [pdm [in_map in_pdm]].
+    apply In_map_iff in in_map as [pdm' [pdm_pdm' pdm'_in_db]].
+    destruct (al_assoc pd exceptions) eqn:A;
+      subst pdm; apply filter_predicate_true in in_pdm;
+      apply negb_true_iff in in_pdm.
+    - apply andb_false_iff in in_pdm. destruct in_pdm as [H|H].
+      + tauto.
+      + apply negb_false_iff in H. apply existsb_exists in H as [sel' [in_l E]].
+        apply Neqb_ok in E. subst. eauto.
+    - eauto.
+  Qed.
+
+  Theorem delete_all_except_preseve_other :
   forall (db:mapping_db) (pd:N) (sel:N) (ko:kernel_object) (f:kernel_object -> bool)
          (exceptions:assoc_list (list N)),
-    has_mapping pd sel ko (remove_all_except f exceptions db) ->
-    f ko = false \/ contains (list N) pd (In sel) exceptions.
-Proof.
-Abort.
-
-Theorem remove_all_except_preseve_other :
-  forall (db:mapping_db) (pd:N) (sel:N) (ko:kernel_object) (f:kernel_object -> bool)
-         (exceptions:assoc_list (list N)),
-    f ko = true ->
+    f ko = false ->
     (has_mapping pd sel ko db <->
-     has_mapping pd sel ko (remove_all_except f exceptions db)).
-Proof.
-Abort.
+     has_mapping pd sel ko (delete_all_except f exceptions db)).
+  Proof.
+    intros db pd sel ko f exceptions ffalse. unfold delete_all_except.
+    split.
+    - unfold has_mapping. unfold contains.
+      destruct 1 as [pdm [in_db in_pdm]]. destruct (al_assoc pd exceptions) eqn:A;
+        eexists; (split;
+          [ apply In_map_iff; rewrite A; eauto
+          | apply al_filter_In; rewrite negb_true_iff; rewrite ffalse; simpl; auto
+          ]).
+    - unfold has_mapping. unfold contains. destruct 1 as [pdm [in_map in_pdm]].
+      apply In_map_iff in in_map. destruct in_map as [pdm' [pdm_pdm' in_db]].
+      destruct (al_assoc pd exceptions);
+        subst pdm; apply al_filter_In in in_pdm; destruct in_pdm; eauto.
+  Qed.
+
+End DeleteAll.
 
 End MappingDB.
